\documentclass[12pt,a4paper]{article}
\usepackage[utf8]{inputenc}
\usepackage{amsmath,multicol}
\usepackage{amsfonts}
\usepackage{amssymb}
\usepackage{graphicx}

\usepackage[%
    left=1.0in,%
    right=1.0in,%
    top=0.8in,%
    bottom=1.0in,%
]{geometry}%

\title{\textbf{Principles of AI Planning
		\\{\Large Exercise Sheet 2}}}
\date{6.11.2019}

\makeatletter
\renewcommand{\@maketitle}
{
	\newpage
	\null
	\vskip 2em%
	\begin{center}%
		{\LARGE \@title \\ \par}%
	\end{center}%
	\par
} \makeatother

\begin{document}
	\begin{flushleft}
		Authors:\\
		Erick Rosete Beas | er165@uni-freiburg.de\\
		Jessica Lizeth Borja Diaz | jb986@uni-freiburg.de\\
	\end{flushleft}
	{\let\newpage\relax\maketitle}
	\begin{center} 
		\large 6.11.2019 
	\end{center}

	\section*{Exercise 2.1 - Effect Normal Form}
	\textbf{a) Transform the operator into ENF}
	
	\begin{align*} 
		\langle\neg e \lor f,
		\\ (a \triangleright (b \triangleright c)) \land
		\\ (\neg d \triangleright c) \land
		\\ (\neg(\neg c \land \neg a) \triangleright (d \land \neg e)) \land 
		\\ (d \triangleright \neg e) \rangle 
	\end{align*} 

\hfill\break
\setlength{\columnsep}{50pt}
\begin{multicols}{2}
	De Morgan's Law
	\begin{align*} 
		\langle\neg e \lor f, 
		\\ (a \triangleright (b \triangleright c))  \land 
		\\ (\neg d \triangleright c) \land 
		\\ ((c \lor a) \triangleright (d \land \neg e)) \land 
		\\ (d \triangleright \neg e) \rangle
	\end{align*} 

	(7)
	\begin{align*} 
		\langle\neg e \lor f, 
		\\ ((a \land b) \triangleright c))  \land 
		\\ (\neg d \triangleright c) \land 
		\\ ((c \lor a) \triangleright (d \land \neg e)) \land 
		\\ (d \triangleright \neg e) \rangle
	\end{align*} 
	
	(9)
	\begin{align*} 
		\langle\neg e \lor f, 
		\\ ((a \land b \lor \neg d) \triangleright c) \land 
		\\ ((c \lor a) \triangleright (d \land \neg e)) \land 
		\\ (d \triangleright \neg e) \rangle
	\end{align*} 
	
	(8)
	\begin{align*} 
		\langle\neg e \lor f,
		\\ ((a \land b \lor \neg d) \triangleright c) \land 
		\\ ((c \lor a) \triangleright d) \land 
		\\((c \lor a) \triangleright \neg e) \land 
		\\(d \triangleright \neg e) \rangle
	\end{align*} 

	(9)
	\begin{align*} 
		\langle\neg e \lor f, 
		\\ ((a \land b \lor \neg d) \triangleright c) \land 
		\\ ((c \lor a) \triangleright d) \land 
		\\ ((c \lor a \lor d) \triangleright \neg e) \rangle
	\end{align*}
\end{multicols}

	\hfill\break
	\textbf{b) Transform the operator into positive normal form}
	\begin{align*} 
		\langle\neg e \lor f, 
		\\ ((a \land b \lor \neg d) \triangleright c) \land 
		\\ ((c \lor a) \triangleright d) \land 
		\\ ((c \lor a \lor d) \triangleright \neg e) \rangle
	\end{align*} 

\hfill\break
\setlength{\columnsep}{50pt}
\begin{multicols}{2}
\noindent First we identify the negative atom $\neg e$ and we change it for $\hat{e}$
	\begin{align*} 
		\langle \hat{e} \lor f, 
		\\ ((a \land b \lor \neg d) \triangleright c) \land 
		\\ ((c \lor a) \triangleright d) \land 
		\\ ((c \lor a \lor d) \triangleright \neg e) \rangle
	\end{align*} 
	We change effect $\neg e$ for $\neg{e} \land \hat{e}$
	\begin{align*} 
		\langle \hat{e} \lor f, 
		\\ ((a \land b \lor \neg d) \triangleright c) \land 
		\\ ((c \lor a) \triangleright d) \land 
		\\ ((c \lor a \lor d) \triangleright (\neg{e} \land \hat{e})) \rangle
	\end{align*} 
	We identify the negative atom $\neg d$ and we change it for $\hat{d}$.
	\begin{align*} 
		\langle \hat{e} \lor f, 
		\\ ((a \land b \lor \hat{d}) \triangleright c) \land 
		\\ ((c \lor a) \triangleright d) \land 
		\\ ((c \lor a \lor d) \triangleright (\neg{e} \land \hat{e})) \rangle
	\end{align*} 
	We change effect $d$ for $d \land \neg \hat{d}$
	\begin{align*} 
		\langle \hat{e} \lor f, 
		\\ ((a \land b \lor \hat{d}) \triangleright c) \land 
		\\ ((c \lor a) \triangleright (d \land \neg \hat{d})) \land 
		\\ ((c \lor a \lor d) \triangleright (\neg{e} \land \hat{e})) \rangle
	\end{align*} 		
	(8)
	\begin{align*} 
		\langle \hat{e} \lor f, 
		\\ ((a \land b \lor \hat{d}) \triangleright c) \land 
		\\ ((c \lor a) \triangleright d) \land 
		\\ ((c \lor a) \triangleright \neg\hat{d}) \land 
		\\ ((c \lor a \lor d) \triangleright (\neg{e} \land \hat{e}) \rangle
	\end{align*} 
	(8)
	\begin{align*} 
		\langle \hat{e} \lor f, 
		\\ ((a \land b \lor \hat{d}) \triangleright c) \land 
		\\ ((c \lor a) \triangleright d) \land 
		\\ ((c \lor a) \triangleright \neg\hat{d}) \land 
		\\ ((c \lor a \lor d) \triangleright \neg{e}) \land 
		\\ ((c \lor a \lor d) \triangleright \hat{e}) \rangle
	\end{align*} 
\end{multicols}

\end{document}